Represent polynomials by ordered associative lists

thys/Groebner_Bases/Algorithm_Schema_Impl.thy
@@ -3,84 +3,46 @@
 section \<open>Code Equations and Useful Functions related to the Computation of Gr\"obner Bases\<close>
 
 theory Algorithm_Schema_Impl
-  imports Algorithm_Schema "Polynomials.MPoly_Type_Class_FMap"
+  imports Algorithm_Schema Polynomials.MPoly_Type_Class_OAlist
 begin
 
-definition keys_list :: "('a \<times> 'b::zero) list \<Rightarrow> 'a list"
-  where "keys_list xs = map fst [x\<leftarrow>AList.clearjunk xs. snd x \<noteq> 0]"
-
-lemma distinct_keys_list: "distinct (keys_list xs)"
-  unfolding keys_list_def using distinct_clearjunk by (rule distinct_map_filter)
-
-lemma compute_keys_alt [code]: "keys (Pm_fmap (fmap_of_list xs)) = set (keys_list xs)"
-proof (simp add: compute_keys_pp clearjunk0_def fmlookup_of_list fmdom'_alt_def fset_of_list.rep_eq
-      keys_list_def)
-  show "{x. map_of xs x \<noteq> Some 0} \<inter> fst ` set xs = fst ` {x \<in> set (AList.clearjunk xs). snd x \<noteq> 0}"
-      (is "?l = ?r")
-  proof
-    show "?l \<subseteq> ?r"
-    proof (rule, simp, elim conjE)
-      fix t
-      assume "map_of xs t \<noteq> Some 0" and "t \<in> fst ` set xs"
-      hence "map_of (AList.clearjunk xs) t \<noteq> Some 0" and "t \<in> fst ` set (AList.clearjunk xs)"
-        by (simp_all add: map_of_clearjunk dom_clearjunk)
-      then obtain c where "(t, c) \<in> set (AList.clearjunk xs)" and "c \<noteq> 0"
-        by (metis domD dom_map_of_conv_image_fst map_of_SomeD)
-      hence "(t, c) \<in> {x \<in> set (AList.clearjunk xs). snd x \<noteq> 0}" by simp
-      thus "t \<in> fst ` {x \<in> set (AList.clearjunk xs). snd x \<noteq> 0}" by force
-    qed
-  next
-    show "?r \<subseteq> ?l"
-    proof (rule, simp)
-      fix t
-      assume "t \<in> fst ` {x \<in> set (AList.clearjunk xs). snd x \<noteq> 0}"
-      then obtain c where "(t, c) \<in> {x \<in> set (AList.clearjunk xs). snd x \<noteq> 0}" by fastforce
-      hence 1: "(t, c) \<in> set (AList.clearjunk xs)" and "c \<noteq> 0" by simp_all
-      from 1 have "map_of (AList.clearjunk xs) t = Some c" by simp
-      hence "map_of xs t = Some c" by (simp only: map_of_clearjunk)
-      with \<open>c \<noteq> 0\<close> have "map_of xs t \<noteq> Some 0" by simp
-      moreover from 1 have "t \<in> fst ` set xs"
-      proof -
-        from 1 have "t \<in> fst ` set (AList.clearjunk xs)" by force
-        thus ?thesis by (simp only: dom_clearjunk)
-      qed
-      ultimately show "map_of xs t \<noteq> Some 0 \<and> t \<in> fst ` set xs" ..
-    qed
-  qed
-qed
-
-lemma compute_card_keys [code]:
-  "card_keys (Pm_fmap (fmap_of_list xs)) = length [x\<leftarrow>AList.clearjunk xs . snd x \<noteq> 0]"
+lemma card_keys_MP_oalist [code]: "card_keys (MP_oalist xs) = length (fst (list_of_oalist_ntm xs))"
 proof -
-  from distinct_keys_list have "card (set (keys_list xs)) = length (keys_list xs)"
-    by (rule distinct_card)
-  also have "... = length [x\<leftarrow>AList.clearjunk xs . snd x \<noteq> 0]" by (simp add: keys_list_def)
-  finally show ?thesis by (simp only: card_keys_def o_def compute_keys_alt)
+  let ?rel = "ko.lt (key_order_of_nat_term_order_inv (snd (list_of_oalist_ntm xs)))"
+  have "irreflp ?rel" by (simp add: irreflp_def)
+  moreover have "transp ?rel" by (simp add: lt_of_nat_term_order_alt)
+  ultimately have *: "distinct (map fst (fst (list_of_oalist_ntm xs)))" using oa_ntm.list_of_oalist_sorted
+    by (rule distinct_sorted_wrt_irrefl)
+  have "card_keys (MP_oalist xs) = length (map fst (fst (list_of_oalist_ntm xs)))"
+    by (simp only: card_keys_def keys_MP_oalist image_set o_def oa_ntm.sorted_domain_def[symmetric],
+        rule distinct_card, fact *)
+  also have "... = length (fst (list_of_oalist_ntm xs))" by simp
+  finally show ?thesis .
 qed
 
 subsection \<open>Generating Cyclic Polynomials\<close>
 
-definition cycl_pp :: "nat \<Rightarrow> nat \<Rightarrow> nat \<Rightarrow> (nat \<Rightarrow>\<^sub>0 nat)"
+definition cycl_pp :: "nat \<Rightarrow> nat \<Rightarrow> nat \<Rightarrow> (nat, nat) pp"
   where "cycl_pp n d i = sparse\<^sub>0 (map (\<lambda>k. (modulo (k + i) n, 1)) [0..<d])"
 
-definition cyclic :: "nat \<Rightarrow> ((nat \<Rightarrow>\<^sub>0 nat) \<Rightarrow>\<^sub>0 'a::{zero,one,uminus}) list"
-  where "cyclic n =
+definition cyclic :: "(nat, nat) pp nat_term_order \<Rightarrow> nat \<Rightarrow> ((nat, nat) pp \<Rightarrow>\<^sub>0 'a::{zero,one,uminus}) list"
+  where "cyclic to n =
             (let xs = [0..<n] in
-              (map (\<lambda>d. sparse\<^sub>0 (map (\<lambda>i. (cycl_pp n d i, 1)) xs)) [1..<n]) @ [sparse\<^sub>0 [(cycl_pp n n 0, 1), (0, -1)]]
+              (map (\<lambda>d. distr\<^sub>0 to (map (\<lambda>i. (cycl_pp n d i, 1)) xs)) [1..<n]) @ [distr\<^sub>0 to [(cycl_pp n n 0, 1), (0, -1)]]
             )"
 
 text \<open>\<open>cyclic n\<close> is a system of \<open>n\<close> polynomials in \<open>n\<close> indeterminates, with maximum degree \<open>n\<close>.\<close>
 
 subsection \<open>Generating Katsura Polynomials\<close>
 
-definition Katsura_poly :: "nat \<Rightarrow> nat \<Rightarrow> ((nat \<Rightarrow>\<^sub>0 nat) \<Rightarrow>\<^sub>0 rat)"
-  where "Katsura_poly n i =
-            (\<Sum>j=-(int n)..<(int n) + 1 - i. Var\<^sub>0 (nat (abs j)) * Var\<^sub>0 (nat (abs j + i))) - Var\<^sub>0 i"
+definition Katsura_poly :: "(nat, nat) pp nat_term_order \<Rightarrow> nat \<Rightarrow> nat \<Rightarrow> ((nat, nat) pp \<Rightarrow>\<^sub>0 rat)"
+  where "Katsura_poly to n i =
+            change_ord to ((\<Sum>j=-(int n)..<(int n) + 1 - i. V\<^sub>0 (nat (abs j)) * V\<^sub>0 (nat (abs j + i))) - V\<^sub>0 i)"
 
-definition Katsura :: "nat \<Rightarrow> ((nat \<Rightarrow>\<^sub>0 nat) \<Rightarrow>\<^sub>0 rat) list"
-  where "Katsura n =
+definition Katsura :: "(nat, nat) pp nat_term_order \<Rightarrow> nat \<Rightarrow> ((nat, nat) pp \<Rightarrow>\<^sub>0 rat) list"
+  where "Katsura to n =
           (let xs = [0..<n] in
-            (sparse\<^sub>0 ((sparse\<^sub>0 [(0, 1)], 1) # (map (\<lambda>i. (sparse\<^sub>0 [(Suc i, 1)], 2)) xs) @ [(0, -1)])) # (map (Katsura_poly n) xs)
+            (distr\<^sub>0 to ((sparse\<^sub>0 [(0, 1)], 1) # (map (\<lambda>i. (sparse\<^sub>0 [(Suc i, 1)], 2)) xs) @ [(0, -1)])) # (map (Katsura_poly to n) xs)
           )"
 
 text \<open>\<open>Katsura n\<close> is a system of \<open>n + 1\<close> polynomials in \<open>n + 1\<close> indeterminates, with maximum degree \<open>2\<close>.\<close>
