thys/Groebner_Bases/F4_Examples.thy
@@ -3,19 +3,67 @@
 section \<open>Sample Computations with the F4 Algorithm\<close>
 
 theory F4_Examples
-  imports F4 Algorithm_Schema_Impl Jordan_Normal_Form.Gauss_Jordan_IArray_Impl
+  imports F4 Algorithm_Schema_Impl Jordan_Normal_Form.Gauss_Jordan_IArray_Impl Code_Target_Rat
 begin
 
 text \<open>We only consider scalar polynomials here, but vector-polynomials could be handled, too.\<close>
 
-lemma (in ordered_term) compute_keys_to_list [code]:
-  "keys_to_list (Pm_fmap (fmap_of_list xs)) = rev (ord_term_lin.sort (keys_list xs))"
-  by (simp add: keys_to_list_def compute_keys_alt pps_to_list_def distinct_keys_list
-        distinct_remdups_id ord_term_lin.sorted_list_of_set_sort_remdups)
+subsection \<open>Preliminaries\<close>
 
-lemma (in term_powerprod) compute_list_to_poly [code]: "list_to_poly ts cs = sparse\<^sub>0 (zip ts cs)"
-  by (rule poly_mapping_eqI, simp add: lookup_list_to_poly sparse\<^sub>0_def list_to_fun_def
-      fmlookup_default_def fmlookup_of_list)
+primrec remdups_wrt_rev :: "('a \<Rightarrow> 'b) \<Rightarrow> 'a list \<Rightarrow> 'b list \<Rightarrow> 'a list" where
+  "remdups_wrt_rev f [] vs = []" |
+  "remdups_wrt_rev f (x # xs) vs =
+    (let fx = f x in if List.member vs fx then remdups_wrt_rev f xs vs else x # (remdups_wrt_rev f xs (fx # vs)))"
+
+lemma remdups_wrt_rev_notin: "v \<in> set vs \<Longrightarrow> v \<notin> f ` set (remdups_wrt_rev f xs vs)"
+proof (induct xs arbitrary: vs)
+  case Nil
+  show ?case by simp
+next
+  case (Cons x xs)
+  from Cons(2) have 1: "v \<notin> f ` set (remdups_wrt_rev f xs vs)" by (rule Cons(1))
+  from Cons(2) have "v \<in> set (f x # vs)" by simp
+  hence 2: "v \<notin> f ` set (remdups_wrt_rev f xs (f x # vs))" by (rule Cons(1))
+  from Cons(2) show ?case by (auto simp: Let_def 1 2 List.member_def)
+qed
+
+lemma distinct_remdups_wrt_rev: "distinct (map f (remdups_wrt_rev f xs vs))"
+proof (induct xs arbitrary: vs)
+  case Nil
+  show ?case by simp
+next
+  case (Cons x xs)
+  show ?case by (simp add: Let_def Cons(1) remdups_wrt_rev_notin)
+qed
+
+lemma map_of_remdups_wrt_rev':
+  "map_of (remdups_wrt_rev fst xs vs) k = map_of (filter (\<lambda>x. fst x \<notin> set vs) xs) k"
+proof (induct xs arbitrary: vs)
+  case Nil
+  show ?case by simp
+next
+  case (Cons x xs)
+  show ?case
+  proof (simp add: Let_def List.member_def Cons, intro impI)
+    assume "k \<noteq> fst x"
+    have "map_of (filter (\<lambda>y. fst y \<noteq> fst x \<and> fst y \<notin> set vs) xs) =
+          map_of (filter (\<lambda>y. fst y \<noteq> fst x) (filter (\<lambda>y. fst y \<notin> set vs) xs))"
+      by (simp only: filter_filter conj_commute)
+    also have "... = map_of (filter (\<lambda>y. fst y \<notin> set vs) xs) |` {y. y \<noteq> fst x}" by (rule map_of_filter)
+    finally show "map_of (filter (\<lambda>y. fst y \<noteq> fst x \<and> fst y \<notin> set vs) xs) k =
+                  map_of (filter (\<lambda>y. fst y \<notin> set vs) xs) k"
+      by (simp add: restrict_map_def \<open>k \<noteq> fst x\<close>)
+  qed
+qed
+
+corollary map_of_remdups_wrt_rev: "map_of (remdups_wrt_rev fst xs []) = map_of xs"
+  by (rule ext, simp add: map_of_remdups_wrt_rev')
+
+lemma (in term_powerprod) compute_list_to_poly [code]:
+  "list_to_poly ts cs = distr\<^sub>0 DRLEX (remdups_wrt_rev fst (zip ts cs) [])"
+  by (rule poly_mapping_eqI,
+      simp add: lookup_list_to_poly list_to_fun_def distr\<^sub>0_def oalist_of_list_ntm_def
+        oa_ntm.lookup_oalist_of_list distinct_remdups_wrt_rev lookup_dflt_def map_of_remdups_wrt_rev)
 
 lemma (in ordered_term) compute_Macaulay_list [code]:
   "Macaulay_list ps =
@@ -36,103 +84,95 @@ derive (no) ccompare rat
 derive (dlist) set_impl rat
 derive (no) cenum rat
 
-subsection \<open>Degree-Reverse-Lexicographic Order\<close>
+subsection \<open>Interpretation\<close>
 
-global_interpretation drlex: gd_powerprod drlex_pm drlex_pm_strict
+global_interpretation punit': gd_powerprod "ord_pp_punit cmp_term" "ord_pp_strict_punit cmp_term"
   rewrites "punit.adds_term = (adds)"
   and "punit.pp_of_term = (\<lambda>x. x)"
   and "punit.component_of_term = (\<lambda>_. ())"
   and "punit.monom_mult = monom_mult_punit"
   and "punit.mult_scalar = mult_scalar_punit"
+  and "punit'.punit.min_term = min_term_punit"
+  and "punit'.punit.lt = lt_punit cmp_term"
+  and "punit'.punit.lc = lc_punit cmp_term"
+  and "punit'.punit.tail = tail_punit cmp_term"
+  and "punit'.punit.ord_p = ord_p_punit cmp_term"
+  and "punit'.punit.ord_strict_p = ord_strict_p_punit cmp_term"
+  and "punit'.punit.keys_to_list = keys_to_list_punit cmp_term"
+  for cmp_term :: "('a::nat, 'b::{nat,add_wellorder}) pp nat_term_order"
 
-  defines min_term_scalar_drlex = drlex.punit.min_term
-  and lt_scalar_drlex = drlex.punit.lt
-  and max_scalar_drlex = drlex.ordered_powerprod_lin.max
-  and max_list_scalar_drlex = drlex.ordered_powerprod_lin.max_list
-  and list_max_scalar_drlex = drlex.punit.list_max
-  and higher_scalar_drlex = drlex.punit.higher
-  and lower_scalar_drlex = drlex.punit.lower
-  and lc_scalar_drlex = drlex.punit.lc
-  and tail_scalar_drlex = drlex.punit.tail
-  and ord_p_scalar_drlex = drlex.punit.ord_p
-  and ord_strict_p_scalar_drlex = drlex.punit.ord_strict_p
-  and count_const_lt_components_scalar_drlex = drlex.punit.count_const_lt_components
-  and count_rem_components_scalar_drlex = drlex.punit.count_rem_components
-  and const_lt_component_scalar_drlex = drlex.punit.const_lt_component
-  and full_gb_scalar_drlex = drlex.punit.full_gb
-  and add_pairs_single_sorted_scalar_drlex = drlex.punit.add_pairs_single_sorted
-  and add_pairs_scalar_drlex = drlex.punit.add_pairs
-  and canon_pair_order_aux_scalar_drlex = drlex.punit.canon_pair_order_aux
-  and canon_basis_order_scalar_drlex = drlex.punit.canon_basis_order
-  and new_pairs_sorted_scalar_drlex = drlex.punit.new_pairs_sorted
-  and product_crit_scalar_drlex = drlex.punit.product_crit
-  and chain_ncrit_scalar_drlex = drlex.punit.chain_ncrit
-  and chain_ocrit_scalar_drlex = drlex.punit.chain_ocrit
-  and apply_icrit_scalar_drlex = drlex.punit.apply_icrit
-  and apply_ncrit_scalar_drlex = drlex.punit.apply_ncrit
-  and apply_ocrit_scalar_drlex = drlex.punit.apply_ocrit
-  and part_key_scalar_drlex = drlex.ordered_powerprod_lin.part
-  and sort_key_scalar_drlex = drlex.ordered_powerprod_lin.sort_key
-  and pps_to_list_scalar_drlex = drlex.punit.pps_to_list
-  and keys_to_list_scalar_drlex = drlex.punit.keys_to_list
-  and Keys_to_list_scalar_drlex = drlex.punit.Keys_to_list
-  and sym_preproc_addnew_scalar_drlex = drlex.punit.sym_preproc_addnew
-  and sym_preproc_aux_scalar_drlex = drlex.punit.sym_preproc_aux
-  and sym_preproc_scalar_drlex = drlex.punit.sym_preproc
-  and Macaulay_mat_scalar_drlex = drlex.punit.Macaulay_mat
-  and Macaulay_list_scalar_drlex = drlex.punit.Macaulay_list
-  and pdata_pairs_to_list_scalar_drlex = drlex.punit.pdata_pairs_to_list
-  and Macaulay_red_scalar_drlex = drlex.punit.Macaulay_red
-  and f4_sel_aux_scalar_drlex = drlex.punit.f4_sel_aux
-  and f4_sel_scalar_drlex = drlex.punit.f4_sel
-  and f4_red_aux_scalar_drlex = drlex.punit.f4_red_aux
-  and f4_red_scalar_drlex = drlex.punit.f4_red
-  and f4_aux_scalar_drlex = drlex.punit.f4_aux_punit
-  and f4_scalar_drlex = drlex.punit.f4_punit
-proof -
-  show "gd_powerprod drlex_pm drlex_pm_strict"
-    apply standard
-    subgoal by (simp add: drlex_pm_strict_def)
-    subgoal by (rule drlex_pm_refl)
-    subgoal by (erule drlex_pm_trans, simp)
-    subgoal by (erule drlex_pm_antisym, simp)
-    subgoal by (rule drlex_pm_lin)
-    subgoal by (rule drlex_pm_zero_min)
-    subgoal by (erule drlex_pm_plus_monotone)
-    done
-  show "punit.adds_term = (adds)" by (fact punit_adds_term)
-  show "punit.pp_of_term = (\<lambda>x. x)" by (fact punit_pp_of_term)
-  show "punit.component_of_term = (\<lambda>_. ())" by (fact punit_component_of_term)
-  show "punit.monom_mult = monom_mult_punit" by (simp only: monom_mult_punit_def)
-  show "punit.mult_scalar = mult_scalar_punit" by (simp only: mult_scalar_punit_def)
-qed
+  defines max_punit = punit'.ordered_powerprod_lin.max
+  and max_list_punit = punit'.ordered_powerprod_lin.max_list
+  and find_adds_punit = punit'.punit.find_adds
+  and trd_aux_punit = punit'.punit.trd_aux
+  and trd_punit = punit'.punit.trd
+  and spoly_punit = punit'.punit.spoly
+  and count_const_lt_components_punit = punit'.punit.count_const_lt_components
+  and count_rem_components_punit = punit'.punit.count_rem_components
+  and const_lt_component_punit = punit'.punit.const_lt_component
+  and full_gb_punit = punit'.punit.full_gb
+  and add_pairs_single_sorted_punit = punit'.punit.add_pairs_single_sorted
+  and add_pairs_punit = punit'.punit.add_pairs
+  and canon_pair_order_aux_punit = punit'.punit.canon_pair_order_aux
+  and canon_basis_order_punit = punit'.punit.canon_basis_order
+  and new_pairs_sorted_punit = punit'.punit.new_pairs_sorted
+  and product_crit_punit = punit'.punit.product_crit
+  and chain_ncrit_punit = punit'.punit.chain_ncrit
+  and chain_ocrit_punit = punit'.punit.chain_ocrit
+  and apply_icrit_punit = punit'.punit.apply_icrit
+  and apply_ncrit_punit = punit'.punit.apply_ncrit
+  and apply_ocrit_punit = punit'.punit.apply_ocrit
+  and Keys_to_list_punit = punit'.punit.Keys_to_list
+  and sym_preproc_addnew_punit = punit'.punit.sym_preproc_addnew
+  and sym_preproc_aux_punit = punit'.punit.sym_preproc_aux
+  and sym_preproc_punit = punit'.punit.sym_preproc
+  and Macaulay_mat_punit = punit'.punit.Macaulay_mat
+  and Macaulay_list_punit = punit'.punit.Macaulay_list
+  and pdata_pairs_to_list_punit = punit'.punit.pdata_pairs_to_list
+  and Macaulay_red_punit = punit'.punit.Macaulay_red
+  and f4_sel_aux_punit = punit'.punit.f4_sel_aux
+  and f4_sel_punit = punit'.punit.f4_sel
+  and f4_red_aux_punit = punit'.punit.f4_red_aux
+  and f4_red_punit = punit'.punit.f4_red
+  and f4_aux_punit = punit'.punit.f4_aux_punit
+  and f4_punit = punit'.punit.f4_punit
+  subgoal by (fact gd_powerprod_ord_pp_punit)
+  subgoal by (fact punit_adds_term)
+  subgoal by (simp add: id_def)
+  subgoal by (fact punit_component_of_term)
+  subgoal by (simp only: monom_mult_punit_def)
+  subgoal by (simp only: mult_scalar_punit_def)
+  subgoal using min_term_punit_def by fastforce
+  subgoal by (simp only: lt_punit_def ord_pp_punit_alt)
+  subgoal by (simp only: lc_punit_def ord_pp_punit_alt)
+  subgoal by (simp only: tail_punit_def ord_pp_punit_alt)
+  subgoal by (simp only: ord_p_punit_def ord_pp_strict_punit_alt)
+  subgoal by (simp only: ord_strict_p_punit_def ord_pp_strict_punit_alt)
+  subgoal by (simp only: keys_to_list_punit_def ord_pp_punit_alt) 
+  done
 
-subsubsection \<open>Computations\<close>
+subsection \<open>Computations\<close>
 
 experiment begin interpretation trivariate\<^sub>0_rat .
 
 lemma
-  "lt_scalar_drlex (X\<^sup>2 * Z ^ 3 + 3 * X\<^sup>2 * Y) = sparse\<^sub>0 [(0, 2), (2, 3)]"
+  "lt_punit DRLEX (X\<^sup>2 * Z ^ 3 + 3 * X\<^sup>2 * Y) = sparse\<^sub>0 [(0, 2), (2, 3)]"
   by eval
 
 lemma
-  "lc_scalar_drlex (X\<^sup>2 * Z ^ 3 + 3 * X\<^sup>2 * Y) = 1"
+  "lc_punit DRLEX (X\<^sup>2 * Z ^ 3 + 3 * X\<^sup>2 * Y) = 1"
   by eval
 
 lemma
-  "tail_scalar_drlex (X\<^sup>2 * Z ^ 3 + 3 * X\<^sup>2 * Y) = 3 * X\<^sup>2 * Y"
+  "tail_punit DRLEX (X\<^sup>2 * Z ^ 3 + 3 * X\<^sup>2 * Y) = 3 * X\<^sup>2 * Y"
   by eval
 
 lemma
-  "higher_scalar_drlex (X\<^sup>2 * Z ^ 3 + 3 * X\<^sup>2 * Y) (sparse\<^sub>0 [(0, 2)]) = X\<^sup>2 * Z ^ 3 + 3 * X\<^sup>2 * Y"
+  "ord_strict_p_punit DRLEX (X\<^sup>2 * Z ^ 4 - 2 * Y ^ 3 * Z\<^sup>2) (X\<^sup>2 * Z ^ 7 + 2 * Y ^ 3 * Z\<^sup>2)"
   by eval
 
 lemma
-  "ord_strict_p_scalar_drlex (X\<^sup>2 * Z ^ 4 - 2 * Y ^ 3 * Z\<^sup>2) (X\<^sup>2 * Z ^ 7 + 2 * Y ^ 3 * Z\<^sup>2)"
-  by eval
-
-lemma
-  "f4_scalar_drlex
+  "f4_punit DRLEX
     [
      (X\<^sup>2 * Z ^ 4 - 2 * Y ^ 3 * Z\<^sup>2, ()),
      (Y\<^sup>2 * Z + 2 * Z ^ 3, ())
@@ -146,7 +186,7 @@ lemma
   by eval
 
 lemma
-  "f4_scalar_drlex
+  "f4_punit DRLEX
     [
      (X\<^sup>2 + Y\<^sup>2 + Z\<^sup>2 - 1, ()),
      (X * Y - Z - 1, ()),
@@ -160,8 +200,8 @@ lemma
 
 end
 
-value [code] "length (f4_scalar_drlex (map (\<lambda>p. (p, ())) ((cyclic 4)::(_ \<Rightarrow>\<^sub>0 rat) list)) ())"
+value [code] "length (f4_punit DRLEX (map (\<lambda>p. (p, ())) ((cyclic DRLEX 4)::(_ \<Rightarrow>\<^sub>0 rat) list)) ())"
 
-value [code] "length (f4_scalar_drlex (map (\<lambda>p. (p, ())) (Katsura 2)) ())"
+value [code] "length (f4_punit DRLEX (map (\<lambda>p. (p, ())) (Katsura DRLEX 2)) ())"
 
 end (* theory *)
