thys/Groebner_Bases/Reduced_GB_Examples.thy
@@ -1,5 +1,9 @@
+(* Author: Alexander Maletzky *)
+
+section \<open>Sample Computations of Reduced Gr\"obner Bases\<close>
+
 theory Reduced_GB_Examples
-  imports Buchberger Reduced_GB Polynomials.MPoly_Type_Class_FMap
+  imports Buchberger Reduced_GB Polynomials.MPoly_Type_Class_OAlist Code_Target_Rat
 begin
 
 context gd_term
@@ -15,78 +19,71 @@ end
 
 text \<open>We only consider scalar polynomials here, but vector-polynomials could be handled, too.\<close>
 
-global_interpretation drlex: gd_powerprod drlex_pm drlex_pm_strict
+global_interpretation punit': gd_powerprod "ord_pp_punit cmp_term" "ord_pp_strict_punit cmp_term"
   rewrites "punit.adds_term = (adds)"
   and "punit.pp_of_term = (\<lambda>x. x)"
   and "punit.component_of_term = (\<lambda>_. ())"
   and "punit.monom_mult = monom_mult_punit"
   and "punit.mult_scalar = mult_scalar_punit"
+  and "punit'.punit.min_term = min_term_punit"
+  and "punit'.punit.lt = lt_punit cmp_term"
+  and "punit'.punit.lc = lc_punit cmp_term"
+  and "punit'.punit.tail = tail_punit cmp_term"
+  and "punit'.punit.ord_p = ord_p_punit cmp_term"
+  and "punit'.punit.ord_strict_p = ord_strict_p_punit cmp_term"
+  for cmp_term :: "('a::nat, 'b::{nat,add_wellorder}) pp nat_term_order"
 
-  defines min_term_scalar_drlex = drlex.punit.min_term
-  and lt_scalar_drlex = drlex.punit.lt
-  and max_scalar_drlex = drlex.ordered_powerprod_lin.max
-  and list_max_scalar_drlex = drlex.punit.list_max
-  and higher_scalar_drlex = drlex.punit.higher
-  and lower_scalar_drlex = drlex.punit.lower
-  and lc_scalar_drlex = drlex.punit.lc
-  and tail_scalar_drlex = drlex.punit.tail
-  and ord_p_scalar_drlex = drlex.punit.ord_p
-  and ord_strict_p_scalar_drlex = drlex.punit.ord_strict_p
-  and find_adds_scalar_drlex = drlex.punit.find_adds
-  and trd_aux_scalar_drlex = drlex.punit.trd_aux
-  and trd_scalar_drlex = drlex.punit.trd
-  and spoly_scalar_drlex = drlex.punit.spoly
-  and count_const_lt_components_scalar_drlex = drlex.punit.count_const_lt_components
-  and count_rem_components_scalar_drlex = drlex.punit.count_rem_components
-  and const_lt_component_scalar_drlex = drlex.punit.const_lt_component
-  and full_gb_scalar_drlex = drlex.punit.full_gb
-  and add_pairs_single_sorted_scalar_drlex = drlex.punit.add_pairs_single_sorted
-  and add_pairs_scalar_drlex = drlex.punit.add_pairs
-  and canon_pair_order_aux_scalar_drlex = drlex.punit.canon_pair_order_aux
-  and canon_basis_order_scalar_drlex = drlex.punit.canon_basis_order
-  and new_pairs_sorted_scalar_drlex = drlex.punit.new_pairs_sorted
-  and product_crit_scalar_drlex = drlex.punit.product_crit
-  and chain_ncrit_scalar_drlex = drlex.punit.chain_ncrit
-  and chain_ocrit_scalar_drlex = drlex.punit.chain_ocrit
-  and apply_icrit_scalar_drlex = drlex.punit.apply_icrit
-  and apply_ncrit_scalar_drlex = drlex.punit.apply_ncrit
-  and apply_ocrit_scalar_drlex = drlex.punit.apply_ocrit
-  and trdsp_scalar_drlex = drlex.punit.trdsp
-  and gb_sel_scalar_drlex = drlex.punit.gb_sel
-  and gb_red_aux_scalar_drlex = drlex.punit.gb_red_aux
-  and gb_red_scalar_drlex = drlex.punit.gb_red
-  and gb_aux_scalar_drlex = drlex.punit.gb_aux_punit
-  and gb_scalar_drlex = drlex.punit.gb_punit
-  and comp_min_basis_pre_scalar_drlex = drlex.punit.comp_min_basis_pre
-  and comp_min_basis_aux_scalar_drlex = drlex.punit.comp_min_basis_aux
-  and comp_min_basis_scalar_drlex = drlex.punit.comp_min_basis
-  and comp_red_basis_aux_scalar_drlex = drlex.punit.comp_red_basis_aux
-  and comp_red_basis_scalar_drlex = drlex.punit.comp_red_basis
-  and monic_scalar_drlex = drlex.punit.monic
-  and comp_red_monic_basis_scalar_drlex = drlex.punit.comp_red_monic_basis
-  and rgb_scalar_drlex = drlex.punit.rgb_punit
-proof -
-  show "gd_powerprod drlex_pm drlex_pm_strict"
-    apply standard
-    subgoal by (simp add: drlex_pm_strict_def)
-    subgoal by (rule drlex_pm_refl)
-    subgoal by (erule drlex_pm_trans, simp)
-    subgoal by (erule drlex_pm_antisym, simp)
-    subgoal by (rule drlex_pm_lin)
-    subgoal by (rule drlex_pm_zero_min)
-    subgoal by (erule drlex_pm_plus_monotone)
-    done
-  show "punit.adds_term = (adds)" by (fact punit_adds_term)
-  show "punit.pp_of_term = (\<lambda>x. x)" by (fact punit_pp_of_term)
-  show "punit.component_of_term = (\<lambda>_. ())" by (fact punit_component_of_term)
-  show "punit.monom_mult = monom_mult_punit" by (simp only: monom_mult_punit_def)
-  show "punit.mult_scalar = mult_scalar_punit" by (simp only: mult_scalar_punit_def)
-qed
+  defines find_adds_punit = punit'.punit.find_adds
+  and trd_aux_punit = punit'.punit.trd_aux
+  and trd_punit = punit'.punit.trd
+  and spoly_punit = punit'.punit.spoly
+  and count_const_lt_components_punit = punit'.punit.count_const_lt_components
+  and count_rem_components_punit = punit'.punit.count_rem_components
+  and const_lt_component_punit = punit'.punit.const_lt_component
+  and full_gb_punit = punit'.punit.full_gb
+  and add_pairs_single_sorted_punit = punit'.punit.add_pairs_single_sorted
+  and add_pairs_punit = punit'.punit.add_pairs
+  and canon_pair_order_aux_punit = punit'.punit.canon_pair_order_aux
+  and canon_basis_order_punit = punit'.punit.canon_basis_order
+  and new_pairs_sorted_punit = punit'.punit.new_pairs_sorted
+  and product_crit_punit = punit'.punit.product_crit
+  and chain_ncrit_punit = punit'.punit.chain_ncrit
+  and chain_ocrit_punit = punit'.punit.chain_ocrit
+  and apply_icrit_punit = punit'.punit.apply_icrit
+  and apply_ncrit_punit = punit'.punit.apply_ncrit
+  and apply_ocrit_punit = punit'.punit.apply_ocrit
+  and trdsp_punit = punit'.punit.trdsp
+  and gb_sel_punit = punit'.punit.gb_sel
+  and gb_red_aux_punit = punit'.punit.gb_red_aux
+  and gb_red_punit = punit'.punit.gb_red
+  and gb_aux_punit = punit'.punit.gb_aux_punit
+  and gb_punit = punit'.punit.gb_punit \<comment>\<open>Faster, because incorporates product criterion.\<close>
+  and comp_min_basis_pre_punit = punit'.punit.comp_min_basis_pre
+  and comp_min_basis_aux_punit = punit'.punit.comp_min_basis_aux
+  and comp_min_basis_punit = punit'.punit.comp_min_basis
+  and comp_red_basis_aux_punit = punit'.punit.comp_red_basis_aux
+  and comp_red_basis_punit = punit'.punit.comp_red_basis
+  and monic_punit = punit'.punit.monic
+  and comp_red_monic_basis_punit = punit'.punit.comp_red_monic_basis
+  and rgb_punit = punit'.punit.rgb_punit
+  subgoal by (fact gd_powerprod_ord_pp_punit)
+  subgoal by (fact punit_adds_term)
+  subgoal by (simp add: id_def)
+  subgoal by (fact punit_component_of_term)
+  subgoal by (simp only: monom_mult_punit_def)
+  subgoal by (simp only: mult_scalar_punit_def)
+  subgoal using min_term_punit_def by fastforce
+  subgoal by (simp only: lt_punit_def ord_pp_punit_alt)
+  subgoal by (simp only: lc_punit_def ord_pp_punit_alt)
+  subgoal by (simp only: tail_punit_def ord_pp_punit_alt)
+  subgoal by (simp only: ord_p_punit_def ord_pp_strict_punit_alt)
+  subgoal by (simp only: ord_strict_p_punit_def ord_pp_strict_punit_alt)
+  done
 
 experiment begin interpretation trivariate\<^sub>0_rat .
 
 lemma
-  "rgb_scalar_drlex
+  "rgb_punit DRLEX
     [
      X ^ 3 - X * Y * Z\<^sup>2,
      Y\<^sup>2 * Z - 1
@@ -100,7 +97,7 @@ lemma
   by eval
 
 lemma
-  "rgb_scalar_drlex
+  "rgb_punit DRLEX
     [
      X\<^sup>2 + Y\<^sup>2 + Z\<^sup>2 - 1,
      X * Y - Z - 1,
