thys/Polynomials/MPoly_Type_Class_FMap.thy
@@ -11,9 +11,9 @@ begin
 text \<open>In this theory, (type class) multivariate polynomials of type
   @{typ "('a, 'b) poly_mapping"} are represented as association lists.\<close>
 
-text \<open>In principle, one could also build upon theory \<open>Polynomials\<close>, although there the representations of
-  power-products and polynomials additionally have to satisfy certain invariants, which we do not
-  require here.\<close>
+text \<open>It is important to note that theory "MPoly_Type_Class_OAlist", which represents polynomials as
+  @{emph \<open>ordered\<close>} associative lists, is much better suited for doing actual computations. This
+  theory is only included for being able to compare the two representations in terms of efficiency.\<close>
 
 subsection \<open>Power Products\<close>
 
